RiscvDialect/proof2.lean
@@ -1,0 +1,234 @@
+import RiscvDialect.RDialect
+import SSA.Projects.InstCombine.LLVM.Semantics
+import SSA.Projects.InstCombine.LLVM.PrettyEDSL
+import SSA.Projects.InstCombine.Refinement
+import SSA.Projects.InstCombine.Tactic
+import SSA.Projects.InstCombine.TacticAuto
+import SSA.Projects.InstCombine.Base
+import SSA.Projects.InstCombine.ForLean
+import Lean
+
+open toRISCV -- the riscv dialect
+open InstCombine (LLVM)
+
+
+/-
+A context refinement is a function that maps each valid RISC-V variable (a de Bruijn index in Δ with type .bv)
+ to a corresponding LLVM variable (a de Bruijn index in Γ with type .bitvec 64).
+-/
+
+
+def CtxtRefines (Γ : Ctxt LLVM.Ty) (Δ : Ctxt RV64.Ty) : Type := -- defining how to the types are mapped between the two contexts
+  (Δ.Var .bv) → Γ.Var (.bitvec 64)
+
+#print CtxtRefines
+
+--def V₁:= (Ctxt.Valuation.ofHVector lh_llvm)
+--def V₂:= (Ctxt.Valuation.ofHVector lh_riscv)
+def LLVMCtxt := Ctxt InstCombine.Ty
+def RISCVCtxt := Ctxt toRISCV.Ty
+
+
+
+--def V₁:= (Ctxt.Valuation.ofHVector lh_llvm)
+--def V₂:= (Ctxt.Valuation.ofHVector lh_riscv)
+
+def toLLVM : RV64.Ty → InstCombine.Ty
+  | .bv => .bitvec 64 -- keep in mind the InstCombine Ty is an otion bit vec
+
+-- this defines how given a riscv context, the corresponding LLVM context should look under equailty assumptions
+def RISCV_to_LLVM_should (B : Ctxt RV64.Ty) : (Ctxt LLVM.Ty) :=
+  Ctxt.map toLLVM B
+
+-- this checks that the LLVM context is exactly what the RISCV context would expect
+def contextCrossDialectEquality1 (A : Ctxt InstCombine.Ty) (B : Ctxt RV64.Ty) : Prop :=
+  (RISCV_to_LLVM_should B) = A
+
+
+-- not sure how to implement this
+def CtxtRefinesFunc (Γ : Ctxt LLVM.Ty) (Δ : Ctxt RV64.Ty) : Type := -- defining how to the types are mapped between the two contexts
+  (Δ.Var .bv) → Γ.Var (.bitvec 64) -- from bit vec to option bit vec
+
+
+structure ValutationRefinesEq {A : Ctxt InstCombine.Ty} {B: Ctxt RV64.Ty} (AV : A.Valuation) (BV : B.Valuation) where
+  f : CtxtRefinesFunc A B
+  val_refines : ∀ (v : B.Var .bv) (x : BitVec 64) , AV (f v) = some x → BV v = x
+
+structure ValuationRefines {Γ : LLVMCtxt} {Δ : RISCVCtxt} (V₁ : Γ.Valuation) (V₂ : Δ.Valuation) where
+  ctxtRefines : CtxtRefines Γ Δ -- defining how to values should be mapped, challenge; llvm type is option bc of UB
+  val_refines : ∀ (v : Δ.Var .bv) (x : BitVec 64), V₁ (ctxtRefines v) = some x → V₂ v = x --if the llvm variable has a some value we have the riscv value given
+
+
+
+-- my proposal but not sure of the context refinement
+def CtxtRefinesFuncRiscvToLLVM (Γ : Ctxt LLVM.Ty) (Δ : Ctxt RV64.Ty) : Type := -- defining how to the types are mapped between the two contexts
+ Γ.Var (.bitvec 64) → (Δ.Var .bv)
+-- here then distingguish whether it is a none or some
+
+structure ValuationProposal {Γ : LLVMCtxt} {Δ : RISCVCtxt} (V₁ : Γ.Valuation) (V₂ : Δ.Valuation) where
+f : CtxtRefinesFuncRiscvToLLVM A B
+val_refines : ∀ (v : Γ.Var (.bitvec 64)) (x : BitVec 64), V₁ v = some x → V₂ (f v) = x
+-- if the llvm type is a some then there must be a corresponding value given by the ctxt mapping function
+-- bc here as a next step in the proof i would need to extract what llvm variables where used and
+-- bc the computation returns some would need have the implication that there must be a corresnding reiscv mapping
+
+
+def allVarsRiscv (Δ : Ctxt (toRISCV.Ty)) : List (Δ.Var .bv) :=
+  (List.range Δ.length).map (fun i =>
+    ⟨i, sorry⟩)
+
+def allVarsLLVM (Γ : Ctxt (InstCombine.Ty)) : List (Γ.Var (.bitvec 64)) :=
+  (List.range Γ.length).map (fun i =>
+    ⟨i, sorry⟩)
+
+-- type of var is a DeBruijn index meaning a nat and a proof that the nat has the correspodning type
+def evalContextRiscv (Δ : RISCVCtxt) (V₁ : Δ.Valuation) : List (BitVec 64) :=
+  (allVarsRiscv Δ).map (@V₁ _)
+
+
+-- type of var is a DeBruijn index meaning a nat and a proof that the nat has the correspodning type
+def evalContextLLVM(Γ : Ctxt (InstCombine.Ty)) (V₁ : Γ.Valuation) : List (Option (BitVec 64)) :=
+  (allVarsLLVM Γ).map (@V₁ _)
+
+/-
+List (BitVec 64)
+-/
+
+/-
+structure ValuationRefines {Γ : LLVMCtxt} {Δ : RISCVCtxt} (V₁ : Γ.Valuation) (V₂ : Δ.Valuation) where
+  ctxtRefines : CtxtRefines Γ Δ -- defining how to values should be mapped, challenge; llvm type is option bc of UB
+  val_refines : ∀ (v : Δ.Var .bv) (x : BitVec 64), V₁ (ctxtRefines v) = some x → V₂ v = x
+-/
+
+def convertLLVMContextToRiscv (LLVMVariables : List (Option (BitVec 64))) : List ((BitVec 64)) :=
+  LLVMVariables.foldr (fun x acc =>
+    match x with
+    | some v => v :: acc
+    | none   => acc
+  ) []
+
+def dialectContextTransform2 (Δ : RISCVCtxt) (Γ : LLVMCtxt) (f :RV64.Ty → LLVM.Ty ): Prop :=
+  (Ctxt.map f Δ) = Γ
+/-
+def dialectValuationTransform (Δ : RISCVCtxt) (Γ : LLVMCtxt) (f :RV64.Ty → LLVM.Ty ) : Prop :=
+  (Ctxt.map f Δ) = Γ ∧ Ctxt.map (Ctxt.Valuation Δ RV64TyDenote.toType) Δ
+-/
+
+def dialectValuationTransform (Δ : RISCVCtxt) (Γ : LLVMCtxt) (V₁ : Γ.Valuation) (V₂ : Δ.Valuation): Prop :=
+  convertLLVMContextToRiscv (evalContextLLVM Γ V₁)  = (evalContextRiscv Δ V₂)
+
+structure contextMatch {Γ : LLVMCtxt} {Δ : RISCVCtxt} (V₁ : Γ.Valuation) (V₂ : Δ.Valuation) where
+  ctxtEq :  convertLLVMContextToRiscv (evalContextLLVM Γ V₁)  = (evalContextRiscv Δ V₂)
+
+
+theorem eq_of_contextMatch_of_eq {Γ : LLVMCtxt} {Δ : RISCVCtxt} {V₁ : Γ.Valuation} {V₂ : Δ.Valuation}
+  (h : contextMatch V₁ V₂) (hV₁ : V₁ ⟨i, hiV1⟩ = some x) : V₂ ⟨i, hiV2⟩ = x := sorry
+
+
+def riscv_add :=
+  [RV64_com| {
+    ^entry (%X: !i64, %Y: !i64):
+    %v1 = "RV64.add" (%X, %Y) : (!i64, !i64) -> (!i64)
+    "return" (%v1) : (!i64, !i64) -> ()
+  }]
+
+theorem denote_riscv_add_eq_add (v1 v2 : BitVec 64)
+  (h1 : (V ⟨0, by rfl⟩) = v1)
+  (h2 : (V ⟨1, by rfl⟩) =  v2) :
+  riscv_add.denote V =  (v1 + v2) := by
+unfold riscv_add
+simp_peephole
+simp [HVector.getN, HVector.get]
+repeat rw [Ctxt.Var.last]
+rw [h1] -- TODO: correct normal forms and simprocs
+rw [RV64.RTYPE_pure64_RISCV_ADD]
+rw [BitVec.add_eq]
+congr
+
+def llvm_add :=
+  [llvm(64)| {
+^bb0(%X : i64, %Y : i64):
+      %v1 = llvm.add %Y, %X : i64
+      llvm.return %v1 : i64
+}]
+
+theorem denote_llvm_add_eq_add_of_eq_some_of_eq_some
+  (h1 : (V ⟨0, by rfl⟩) = some v1)
+  (h2 : (V ⟨1, by rfl⟩) = some v2) :
+  llvm_add.denote V = some (v1 + v2) := by
+unfold llvm_add
+simp_peephole
+simp [HVector.getN, HVector.get]
+rw [Ctxt.Var.last]
+rw [h2, h1]
+simp [LLVM.add] -- TODO: non-confluent simp-set.
+rw [LLVM.add?_eq]
+
+theorem denote_llvm_add_eq_none_of_eq_none_left
+  (h1 : (V ⟨0, by rfl⟩) = none) :
+  llvm_add.denote V = none := by
+unfold llvm_add
+simp_peephole
+simp [HVector.getN, HVector.get]
+rw [Ctxt.Var.last]
+rw [h1]
+simp [LLVM.add] -- TODO: non-confluent simp-set.
+
+theorem denote_llvm_add_eq_none_of_eq_none_right
+  (h2 : (V ⟨1, by rfl⟩) = none) :
+  llvm_add.denote V = none := by
+unfold llvm_add
+simp_peephole
+simp [HVector.getN, HVector.get]
+rw [Ctxt.Var.last]
+rw [h2]
+simp [LLVM.add] -- TODO: non-confluent simp-set.
+
+theorem valuation_eq_some_of_llvm_add_denote_eq_some
+  (h : llvm_add.denote V = some x) :
+    ∃ (v1 v2 : BitVec 64),
+      (V ⟨0, by rfl⟩ = some v1) ∧ (V ⟨1, by rfl⟩ = some v2) ∧ (v1 + v2 = x)  := by
+  generalize hv1? : V ⟨0, by rfl⟩ = v1?
+  generalize hv2? : V ⟨1, by rfl⟩ = v2?
+  cases v1?
+  case none =>
+    simp
+    have := denote_llvm_add_eq_none_of_eq_none_left hv1?
+    rw [h] at this
+    contradiction
+  case some v1 =>
+    cases v2?
+    case none =>
+      simp
+      have := denote_llvm_add_eq_none_of_eq_none_right hv2?
+      rw [h] at this
+      contradiction
+    case some v2 =>
+      exists v1
+      exists v2
+      simp
+      have := denote_llvm_add_eq_add_of_eq_some_of_eq_some hv1? hv2?
+      rw [h] at this
+      injection this with this
+      rw [this]
+
+theorem see_LLVM3 (V₁) (V₂) (h : contextMatch V₁ V₂) : -- i know that at core both contexts map to the same values, none values are filitered out
+    ∀ x, (llvm_add.denote V₁ = some x → riscv_add.denote V₂ = x) := by
+    let ⟨val_refines⟩ := h
+    --simp_alive_meta
+    cases h1 :  (llvm_add.denote V₁) with
+    | none =>
+      intros x hx
+      simp at hx
+    | some val =>
+      intros x hx
+      injection hx with hx
+      subst hx
+      have := valuation_eq_some_of_llvm_add_denote_eq_some h1
+      obtain ⟨v1, v2, hv1, hv2, hadd⟩ := this
+      rw [denote_riscv_add_eq_add v1 v2]
+      · rw [hadd]
+      · -- use context match
+        sorry
+      · -- use context match
+        sorry
